Coq/EC/WindowedMulMachine.v
@@ -1,0 +1,2067 @@
+
+Set Implicit Arguments.
+
+(* A machine that can calculate a group multiplication by performing somewhat arbitrary double and add operations.
+We can perform transformations on the machine and show that the result of the calculation is unchanged. This gives
+us a simple way to describe various optimized group multiplication operations. We can start with a program that is
+equivalent to some windowed multiplication operation that was proved correct in GroupMulWNAF. Then we transform 
+the program until it is equivalent to some other operation (e.g. an optimized implementation in code). The transformation
+operations may fail, so it is also necessary to prove that the desired transformations will succeed. *)
+
+Require Import ZArith.BinInt.
+Require Import List.
+Require Import Arith.
+Require Import Arith.Peano_dec.
+Require Import Arith.Compare_dec.
+Require Import Permutation.
+Require Import Nat.
+Require Import micromega.Lia.
+Require Import SetoidClass.
+
+From EC Require Import GroupMulWNAF.
+
+(* A tactic that simplifies hypothesis involving option values*)
+Ltac optSomeInv_1 := 
+  match goal with 
+    | [H : match ?a with | Some _ => _ | None => _ end = Some _ |- _ ] =>
+      case_eq a; [ intro | idtac]; (let v := fresh in intro v; rewrite v in H); [idtac | discriminate]
+    | [H : Some _ = Some _ |- _ ] => inversion H; clear H; subst
+    end.
+
+Ltac optSomeInv := repeat optSomeInv_1.
+
+(* Combine a list of option into an option list *)
+Fixpoint combineOpt(A: Type)(ls : list (option A)) :=
+  match ls with
+  | nil => Some nil
+  | opta :: ls' => 
+    match opta with
+    | None => None
+    | Some a =>
+      match (combineOpt ls') with
+      | None => None
+      | Some ls'' => Some (a :: ls'')
+      end
+    end
+  end.
+
+Theorem combineOpt_perm_ex : forall (A : Type)(ls1 ls2 : list (option A)),
+  Permutation ls1 ls2 ->
+  forall ls1', 
+  combineOpt ls1 = Some ls1' ->
+  exists ls2', 
+  combineOpt ls2 = Some ls2' /\
+  Permutation ls1' ls2'.
+
+  induction 1; intros; simpl in *.
+  inversion H; clear H; subst.
+  exists nil.
+  intuition idtac.
+  econstructor.
+
+  destruct x; simpl in *.
+  remember (combineOpt l) as z.
+  destruct z.
+  inversion H0; clear H0; subst.
+  destruct (IHPermutation l0).
+  reflexivity.
+  intuition idtac.
+  exists (a :: x).
+  rewrite H1.
+  intuition idtac.
+  econstructor.
+  trivial.
+  discriminate.
+  discriminate.
+
+  destruct y; try discriminate.
+  destruct x; try discriminate.
+  remember (combineOpt l) as z1; destruct z1.
+  inversion H; clear H; subst.
+  exists (a0 :: a :: l0).
+  intuition idtac.
+  econstructor.
+  discriminate.
+
+  destruct (IHPermutation1 ls1').
+  trivial.
+  intuition idtac.
+  destruct (IHPermutation2 x).
+  trivial.
+  intuition idtac.
+  exists x0.
+  intuition idtac.
+  econstructor; eauto.
+
+Qed.
+
+(* Select a number of items from a list based on index *)
+Definition multiSelect(A : Type)(ls : list A)(lsn : list nat) : option (list A) :=
+  combineOpt (map (nth_error ls) lsn).
+
+
+Inductive WindowedMultOp :=
+  | wm_Add : nat -> Z -> WindowedMultOp (* wm_Add n z means add z * 2^n to the accumulator *)  
+  | wm_Double : nat -> WindowedMultOp (* Double the value in the accumulator *)
+.
+
+(* Take a list of signed windows and convert them to a program *)
+Fixpoint signedWindowsToProg (ws : list SignedWindow)(n : nat) :=
+  match ws with
+  | nil => nil
+  | w :: ws' => (wm_Add n w) :: (signedWindowsToProg ws' (S n))
+  end.
+
+
+
+(* Operations that preserve the value *)
+
+(* Insert a double at the head of the list and adjust exponents on remaining items *)
+Definition decrExp (n : nat)(p : WindowedMultOp) :=
+  match p with
+  | wm_Add n' w =>
+    if (le_dec n n') then (Some (wm_Add (n' - n) w)) else None
+  | wm_Double n' => Some (wm_Double n')
+  end.
+
+Fixpoint decrExpLs (n : nat)(ps : list WindowedMultOp) :=
+  match ps with
+  | nil => Some nil
+  | p :: ps' =>
+    match (decrExp n p) with
+    | None => None
+    | Some p' => 
+      match (decrExpLs n ps') with
+      | None => None
+      | Some ps'' =>
+        Some (p' :: ps'')
+      end
+    end
+  end.
+
+Definition insertDouble n ps :=
+  match (decrExpLs n ps) with
+  | Some ps' => Some ((wm_Double n) :: ps')
+  | None => None
+  end.
+
+Fixpoint insertDoubleAt d (ls : list WindowedMultOp)(n : nat) : option (list WindowedMultOp) :=
+  match n with
+  | O => (insertDouble d ls)
+  | S n' => 
+    match ls with
+    | nil => None
+    | x :: ls' =>
+      match (insertDoubleAt d ls' n') with
+      | None => None
+      | Some ls'' => Some (x :: ls'')
+      end
+    end
+  end.
+
+Fixpoint insertDoublesAt d ls lsn :=
+  match lsn with
+  | nil => Some ls
+  | n :: lsn' => 
+    match (insertDoubleAt d ls n) with
+    | None => None
+    | Some ls' => insertDoublesAt d ls' lsn'
+    end
+  end.
+
+
+(* We can arbitrarily permute and insert accumulator doublings. If it succeeds, then the value computed 
+by this program will be the same as the basic windowed multiplication. *)
+Definition permuteAndDouble ws d (perm doubles : list nat) :=
+  match (multiSelect (signedWindowsToProg ws 0) perm) with
+  | None => None
+  | Some ps => insertDoublesAt d ps doubles
+  end.
+
+
+Fixpoint decrExpsLs n ps :=
+  match ps with
+  | nil => Some nil
+  | p :: ps' => 
+    match (decrExpsLs n ps') with
+    | None => None
+    | Some x => 
+      match (combineOpt (map (decrExpLs  n) x)) with
+      | None => None
+      | Some x' => Some (p :: x')
+      end
+    end
+  end.
+
+
+(* A specialization of permuteAndDouble that only inserts doublings after each grouping *)
+Definition permuteAndDouble_grouped ws d (perm : list (list nat)) :=
+  match (combineOpt (map (multiSelect (signedWindowsToProg ws 0)) perm)) with
+  | None => None
+  | Some ps => 
+    match (decrExpsLs d ps) with
+    | None => None
+    | Some x => Some (map (fun x=> x ++ (wm_Double d)::nil ) x)
+    end
+  end.
+
+(* Swap the order of two operations *)
+Definition swapPair p1 p2 :=
+  match p1 with
+  | wm_Add n1 z1 =>
+    match p2 with
+    | wm_Add n2 z2 => Some (p2, p1)
+    | wm_Double n2 => 
+      if (le_dec n2 n1) then Some (p2, (wm_Add (n1 - n2) z1)) else None
+    end
+  | wm_Double n1 =>
+    match p2 with
+    | wm_Add n2 z2 => Some ((wm_Add (n1 + n2) z2),  p1)
+    | wm_Double n2 => Some (p2, p1)
+    end
+  end.
+
+Definition swapFront ps := 
+  match ps with 
+  | nil => None
+  | p1 :: ps' =>
+    match ps' with
+    | nil => None
+    | p2 :: ps'' =>
+      match (swapPair p1 p2) with
+      | None => None
+      | Some (a, b) => Some (a :: b ::  ps'')
+      end
+    end
+  end.
+
+(* A predicate stating that a program contains only add operations *)
+Definition AddProg : list WindowedMultOp -> Prop :=
+  Forall (fun x => match x with | wm_Add _ _ => True | _ => False end).
+
+Definition divides x y :=
+  eq_nat_dec (gcd x y) x.
+
+
+(* returns true if v = k*x + y for some k, false otherwise*)
+Definition isMultiple v x y :=
+  if (ge_dec v y) then (if (divides x (v - y)) then true else false) else false.
+
+Fixpoint endIndices_h(A : Type)(ls : list (list A))(x : nat) :=
+    match ls with
+    | nil => nil
+    | a :: ls' => 
+      ((length a) + x)%nat :: (endIndices_h ls' (length a + x))
+    end.
+
+(* insert doublings from back to front so that it doesn't upset earlier indices *)
+Definition endIndices(A : Type)(ls : list (list A)) :=
+  (rev (endIndices_h ls O)).
+
+Theorem isMultiple_true : forall a x b,
+  isMultiple (a * x + b) x b = true.
+
+  intros.
+  unfold isMultiple.
+  destruct (ge_dec (a * x + b) b).
+  rewrite Nat.add_sub.
+  unfold divides.
+  replace (a * x)%nat with (0 + a * x)%nat.
+  rewrite Nat.gcd_add_mult_diag_r.
+  rewrite Nat.gcd_0_r.
+  destruct (Nat.eq_dec x x).
+  trivial.
+  intuition idtac.
+  lia.
+  lia.
+
+Qed.
+
+
+Theorem isMultiple_true_if : forall y x b,
+  isMultiple y x b = true ->
+  exists a, y  = (a * x + b)%nat.
+
+  intros. 
+  unfold isMultiple in *.
+  destruct (ge_dec y b).
+  destruct (eq_nat_dec x O).
+  subst.
+  exists O.
+  simpl.
+  unfold divides in *.
+  destruct (Nat.eq_dec (gcd O (y - b))%nat).
+  apply Nat.gcd_eq_0_r in e.
+  lia.
+  discriminate.
+  exists ((y - b) / x)%nat.
+  unfold divides in *.
+  destruct (Nat.eq_dec (gcd x (y - b)) x).
+  replace ((y - b) / x * x )%nat with ((y - b) / Nat.gcd (y - b) x * x)%nat.
+  rewrite Nat.lcm_equiv2.
+  rewrite Nat.gcd_comm.
+  rewrite e.
+  rewrite Nat.div_mul.
+  lia.
+  trivial.
+  intuition idtac.
+  rewrite Nat.gcd_comm in H0.
+  rewrite H0 in e.
+  lia.
+  rewrite Nat.gcd_comm.
+  rewrite e.
+  reflexivity.  
+  discriminate.
+  discriminate.
+Qed.
+
+Fixpoint lsMultiples(nMax numGroups curGroup : nat) :=
+  match nMax with
+  | O => nil
+  | S nMax' => (lsMultiples nMax' numGroups curGroup) ++ 
+  (if (isMultiple nMax' numGroups curGroup) then nMax'::nil else nil)
+   
+end.
+
+Theorem In_lsMultiples : forall nMax a x b,
+  (b < x)%nat ->
+  (a * x + b < nMax)%nat -> 
+  In (a * x + b)%nat (lsMultiples nMax x b).
+
+  induction nMax; intros; simpl in *.
+  lia.
+  destruct (eq_nat_dec (a*x + b) nMax).
+  subst.
+  apply in_or_app.
+  right.
+  rewrite isMultiple_true.
+  simpl.
+  intuition idtac.
+  apply in_or_app.
+  left.
+  eapply IHnMax.
+  eauto.
+  lia.
+
+Qed.
+
+Theorem In_lsMultiples_if : forall nMax a x b,
+  In a (lsMultiples nMax x b) -> 
+  (a < nMax)%nat.
+
+  induction nMax; intros; simpl in *.
+  intuition idtac.
+  destruct (isMultiple nMax x b); intros.
+  apply in_app_or in H.
+  simpl in *.
+  intuition idtac.
+  eapply IHnMax in H0.
+  lia.
+  subst.
+  lia.   
+  rewrite app_nil_r in *.
+  apply IHnMax in H.
+  lia.
+
+Qed.
+
+Theorem lsMultiples_gcd : forall nw m i, 
+  List.Forall (fun x : nat => Nat.gcd (x - i) m = m) (lsMultiples nw m i).
+
+  induction nw; intros; simpl in *.
+  econstructor.
+  eapply Forall_app.
+  intuition idtac.
+  eauto.
+  case_eq (isMultiple nw m i ); intros.
+  econstructor.
+  unfold isMultiple in *.
+  destruct ( ge_dec nw i). 
+  unfold divides in *.  
+  destruct (Nat.eq_dec (gcd m (nw - i)) m).
+  rewrite Nat.gcd_comm.
+  eauto.
+  discriminate.
+  discriminate.
+  econstructor.
+  econstructor.
+
+Qed.
+
+Theorem lsMultiples_div : forall nw m i, 
+  i < m ->
+  m > 0 ->
+  List.Forall (fun x : nat => Nat.div x m = Nat.div (x - i) m) (lsMultiples nw m i).
+
+  induction nw; intros; simpl in *.
+  econstructor.
+  eapply Forall_app.
+  intuition idtac.
+  eauto.
+  case_eq (isMultiple nw m i ); intros.
+  econstructor.
+  unfold isMultiple in *.
+  destruct (ge_dec nw i ).
+  destruct (divides m (nw - i)); intros.
+  assert (exists y, nw = i + y).
+  exists (nw - i).
+  lia.
+  destruct H2.
+  subst.
+  replace (i + x - i) with x in *.   
+  assert (exists y, x = y * m).
+  exists (Nat.div x m).
+  rewrite <- e at 1.
+  rewrite Nat.mul_comm.
+  rewrite <- Nat.gcd_div_swap.
+  rewrite e.
+  rewrite Nat.mul_comm.
+  rewrite Nat.div_same.
+  lia.
+  lia.
+  destruct H2.
+  subst.
+  rewrite Nat.div_add.
+  rewrite Nat.div_small.
+  rewrite Nat.div_mul.
+  lia.
+  lia.
+  lia.
+  lia.
+  lia.
+  discriminate.
+  discriminate.
+  econstructor.
+  econstructor.
+
+Qed.
+
+Theorem lsMultiples_length_weak : forall nw m i,
+  List.Forall (fun x : nat => x < nw) (lsMultiples nw m i).
+
+  induction nw; intros; simpl in *.
+  econstructor.
+  eapply Forall_app.
+  intuition idtac.
+  eapply Forall_impl; eauto.
+  intuition idtac; lia.
+  case_eq (isMultiple nw m i); intros.
+  unfold isMultiple in *.
+  destruct (ge_dec nw i).
+  econstructor.
+  lia.
+  econstructor.
+  discriminate.
+  econstructor.
+  
+Qed.
+
+
+Fixpoint groupIndices_h(nMax numGroups curGroup : nat) :=
+  match curGroup with
+  | O => nil
+  | S curGroup' => 
+    (groupIndices_h nMax numGroups curGroup') ++ ((lsMultiples nMax numGroups curGroup') :: nil)
+  end.
+
+Theorem flatten_app : forall (A : Type)(ls1 ls2 : list (list A)),
+  flatten (ls1 ++ ls2) = (flatten ls1 ++ flatten ls2).
+
+  induction ls1; intros; simpl in *.
+  reflexivity.
+  rewrite <- app_assoc.
+  f_equal.
+  eauto.
+
+Qed.
+
+Definition groupIndices nMax numGroups :=
+  groupIndices_h nMax numGroups numGroups.
+
+Theorem In_groupIndices_h : forall  b1 b2 a x nMax,
+  (b2 < b1)%nat -> 
+  (b2 < x)%nat ->
+  (a * x + b2 < nMax)%nat -> 
+  In (a * x + b2)%nat  (flatten (groupIndices_h nMax x b1)).
+
+  induction b1; intros; simpl in *.
+  lia.
+  
+  destruct (eq_nat_dec b2 b1).
+  subst.
+  rewrite flatten_app.
+  apply in_or_app.
+  simpl.
+  right.
+  apply in_or_app.
+  left.
+  eapply In_lsMultiples.
+  trivial.
+  trivial.
+  rewrite flatten_app.
+  apply in_or_app.
+  left.
+  eapply IHb1.
+  lia.
+  trivial.
+  trivial.
+Qed.
+
+Theorem In_groupIndices_h_if : forall  b1 a x nMax,
+  In a (flatten (groupIndices_h nMax x b1)) -> 
+  (a < nMax)%nat.
+
+  induction b1; intros; simpl in *.
+  intuition idtac.
+  rewrite flatten_app in *.
+  simpl in *.
+  rewrite app_nil_r in *.
+  assert (In a (flatten (groupIndices_h nMax x b1)) \/ In a (lsMultiples nMax x b1)).
+  eapply in_app_or.
+  eapply H.
+  intuition idtac.
+  eapply IHb1; eauto.
+  eapply In_lsMultiples_if; eauto.
+
+Qed.
+
+Theorem NoDup_app : forall (A : Type)(ls1 ls2 : list A),
+  NoDup ls1 -> 
+  NoDup ls2 -> 
+  (forall a, In a ls1 -> In a ls2 -> False) -> 
+  NoDup (ls1 ++ ls2).
+
+  induction ls1; intros; simpl in *.
+  trivial.
+  inversion H; clear H; subst.
+  eapply (@Permutation_NoDup _ (ls1 ++ (a :: ls2))).
+  eapply Permutation_sym.
+  eapply Permutation_middle.
+  eapply IHls1.
+  trivial.
+  econstructor.
+  intuition idtac.
+  eapply H1.
+  left.
+  reflexivity.
+  trivial.
+  trivial.
+  intuition idtac.
+  inversion H2; clear H2; subst.
+  intuition idtac.
+  eauto.
+
+Qed.
+
+Theorem lsMultiples_NoDup : forall nMax x a,
+  NoDup (lsMultiples nMax x a).
+
+  induction nMax; intros; simpl in *.
+  econstructor.
+  eapply NoDup_app.
+  eauto.
+  destruct (isMultiple nMax x a).
+  econstructor.
+  simpl.
+  intuition idtac.
+  econstructor.
+  econstructor.
+  intros.
+  apply In_lsMultiples_if in H.
+  destruct (isMultiple nMax x a); simpl in *.
+  intuition idtac; subst.
+  lia.
+  intuition idtac.
+
+Qed.
+
+Theorem in_lsMultiples_isMultiple : forall n x a b,
+  In x (lsMultiples n a b) ->
+  exists y, (x = y * a + b)%nat.
+
+  induction n; intros; simpl in *.
+  intuition idtac.
+  apply in_app_or in H.
+  intuition idtac.
+  eauto.
+  case_eq (isMultiple n a b); intros;
+  rewrite H in H0.
+  simpl in *.
+  intuition idtac; subst.
+  apply isMultiple_true_if.
+  trivial.
+  simpl in *; intuition idtac.
+
+Qed.
+
+Theorem in_groupIndices_h_isMultiple : forall b a x nMax,
+  In a (flatten (groupIndices_h nMax x b)) ->
+  exists y b', (b' < b /\ a = y * x + b')%nat.
+
+  induction b; intros; simpl in *.
+  intuition idtac.
+  rewrite flatten_app in *.
+  simpl in *.
+  rewrite app_nil_r in *.
+  apply in_app_or in H.
+  intuition idtac.
+  edestruct IHb.
+  eauto.
+  destruct H.
+  intuition idtac.
+  subst.
+  econstructor.
+  exists x1.
+  intuition idtac.
+  lia.
+  apply in_lsMultiples_isMultiple in H0.
+  destruct H0.
+  subst.
+  econstructor.
+  exists b.
+  intuition idtac.
+  lia.
+
+Qed.
+
+
+Theorem mul_add_mod_ne : forall x a1 a2 b1 b2,
+  (b1 < x)%nat ->
+  (b2 < b1)%nat -> 
+  (a1 * x + b1)%nat = (a2 * x + b2)%nat ->
+  False.
+
+  intros.
+  rewrite Nat.mul_comm in H1.
+  rewrite (Nat.mul_comm a2) in H1.
+  apply Nat.div_mod_unique in H1.
+  intuition idtac.
+  lia.
+  lia.
+  lia.
+
+Qed.
+
+Theorem groupIndices_h_NoDup : forall  b x nMax,
+  (b <= x)%nat -> 
+  NoDup (flatten (groupIndices_h nMax x b)).
+
+  induction b; intros; simpl in *.
+  econstructor.
+  rewrite flatten_app.
+  simpl.
+  rewrite app_nil_r.
+  eapply NoDup_app.
+  eapply IHb.
+  lia.
+  apply lsMultiples_NoDup.
+
+  intros.
+  apply in_lsMultiples_isMultiple in H1.
+  apply in_groupIndices_h_isMultiple in H0.
+  destruct H0.
+  destruct H0.
+  destruct H1.
+  intuition idtac.
+  subst.
+  eapply mul_add_mod_ne; [idtac | idtac | eauto].
+  lia.
+  lia.
+
+Qed.
+
+
+Theorem groupIndices_perm : forall x y,
+  y <> O -> 
+  Permutation (seq 0 x) (flatten (groupIndices x y)).
+
+  intros.
+  eapply NoDup_Permutation.
+  apply seq_NoDup.
+  apply groupIndices_h_NoDup.
+  lia.
+
+  intros.
+  intuition idtac.
+  rewrite (Nat.div_mod_eq x0 y).
+  rewrite Nat.mul_comm.
+  unfold groupIndices.
+  eapply In_groupIndices_h.
+  apply Nat.mod_upper_bound.
+  intuition idtac.
+  apply Nat.mod_upper_bound.
+  intuition idtac.
+  rewrite Nat.mul_comm.
+  rewrite <- (Nat.div_mod_eq x0 y).
+  apply in_seq in H0.
+  lia.
+
+  apply in_seq.
+  apply In_groupIndices_h_if in H0.
+  lia.
+
+Qed.
+
+
+
+Theorem nth_error_skipn_eq : forall n3 (A : Type)(ls : list A) n1,
+  (n3 <= n1)%nat ->
+  nth_error ls n1 = nth_error (skipn n3 ls) (n1 - n3).
+
+  induction n3; intros; simpl in *.
+  rewrite Nat.sub_0_r.
+  reflexivity.
+
+  destruct n1.
+  lia.
+  simpl.
+  
+  destruct ls.
+  symmetry.
+  apply nth_error_None.
+  simpl.
+  lia.
+  eapply IHn3.
+  lia.
+
+Qed.
+
+Theorem nth_error_seq_skipn_eq : forall n2 (A : Type)(ls : list A) n1 n3,
+  (n3 <= n1)%nat ->
+  map (nth_error ls) (seq n1 n2) = map (nth_error (skipn n3 ls)) (seq (n1 - n3) n2).
+
+  induction n2; intros; simpl in *.
+  trivial.
+  f_equal.
+  eapply nth_error_skipn_eq.
+  lia.
+  specialize (IHn2 _ ls (S n1) n3).
+  rewrite IHn2.
+  replace (S n1 - n3)%nat with (S (n1 - n3)).
+  reflexivity.
+  lia.
+  lia.
+Qed.
+
+Theorem combineOpt_map_seq_eq : forall (A : Type)(ls : list A),
+  combineOpt (map (nth_error ls) (seq 0 (length ls))) = Some ls.
+
+  induction ls; intros; simpl in *.
+  reflexivity.
+  rewrite (@nth_error_seq_skipn_eq _ _ _ _ 1%nat).
+  simpl.
+  rewrite IHls.
+  reflexivity.
+  trivial.
+
+Qed.
+
+Theorem multiSelect_perm : forall (A : Type)(ls ls' : list A)(lsn : list nat),
+  Permutation lsn (seq O (length ls)) ->
+  multiSelect ls lsn = Some ls' ->
+  Permutation ls ls'.
+
+  intros.
+  unfold multiSelect in *.
+  assert (combineOpt (map (nth_error ls) (seq 0 (length ls))) = Some ls).
+  apply combineOpt_map_seq_eq.
+
+  eapply combineOpt_perm_ex in H0.
+  destruct H0.
+  intuition idtac.
+  rewrite H1 in H2.
+  inversion H2; clear H2; subst.
+  eapply Permutation_sym.
+  trivial.
+  apply Permutation_map.
+  trivial.
+
+Qed.
+
+Theorem multiSelect_in_range_Some : forall (A : Type)(ls : list A)(lsn : list nat),
+  (forall n, In n lsn -> n < length ls)%nat ->
+  exists ls', multiSelect ls lsn = Some ls'.
+
+  induction lsn; intros; simpl in *.
+  exists nil.
+  reflexivity.
+  edestruct (IHlsn).
+  intros.
+  apply H.
+  intuition idtac.
+  unfold multiSelect in *.
+  simpl.
+  case_eq (nth_error ls a); intros.
+  rewrite H0.
+  econstructor; eauto.
+  apply nth_error_None in H1.
+  specialize (H a).
+  intuition idtac.
+  lia.
+
+Qed.
+
+Theorem multiSelect_perm_Some : forall (A : Type)(ls : list A)(lsn : list nat),
+  Permutation lsn (seq O (length ls)) -> 
+  exists ls', multiSelect ls lsn = Some ls'.
+
+  intros.
+  apply multiSelect_in_range_Some.
+  intros.
+  eapply Permutation_in in H0; eauto.
+  apply in_seq in H0.
+  lia.
+  
+Qed.
+
+
+ Theorem combineOpt_app : forall ( A: Type)(ls1 ls2 : list (option A)),
+  combineOpt (ls1 ++ ls2) = 
+  match (combineOpt ls1) with
+  | Some ls1' => 
+    match (combineOpt ls2) with
+    | Some ls2' => Some (ls1' ++ ls2')
+    | None => None
+    end
+  | None => None
+  end.
+
+  induction ls1; intros; simpl in *.
+  destruct (combineOpt ls2); reflexivity.
+  destruct a.
+  rewrite IHls1.
+  destruct (combineOpt ls1).
+  destruct (combineOpt ls2).
+  simpl.
+  reflexivity.
+  reflexivity.
+  reflexivity.
+  reflexivity.
+Qed.
+
+Theorem combineOpt_id : forall (A : Type)(ls : list A),
+  combineOpt (List.map (fun x => Some x) ls) = Some ls.
+
+  induction ls; intros; simpl in *.
+  reflexivity.
+  rewrite IHls.
+  reflexivity.
+  
+Qed.
+
+Theorem decrExp_0 : forall x,
+  decrExp 0 x = Some x.
+
+  intros.
+  unfold decrExp.
+  destruct x.
+  destruct (Compare_dec.le_dec 0 n).
+  rewrite Nat.sub_0_r.
+  reflexivity.
+  lia.
+  reflexivity.
+
+Qed.
+
+Theorem decrExpLs_0 : forall x,
+  decrExpLs 0 x = Some x.
+
+  induction x; intros; simpl in *.
+  reflexivity.
+  rewrite decrExp_0.
+  rewrite IHx.
+  reflexivity.
+
+Qed.
+
+Theorem combineOpt_map_map : forall (A B C : Type) f1 f2 f3 (ls1 : list A) (ls2: list B) (ls3 : list C),
+  (forall x y, f1 x = Some y -> f3 x = f2 y) ->
+  combineOpt (List.map f1 ls1) = Some ls2 ->
+  combineOpt (List.map f2 ls2) = Some ls3 -> 
+  combineOpt (List.map f3 ls1) = Some ls3.
+
+  induction ls1; intros; simpl in *.
+  inversion H0; clear H0; subst.
+  simpl in *.
+  inversion H1; clear H1; subst.
+  reflexivity.
+  case_eq (f1 a); intros;
+  rewrite H2 in H0.
+  case_eq (combineOpt (List.map f1 ls1)); intros;
+  rewrite H3 in H0.
+  inversion H0; clear H0; subst.
+  simpl in *.
+  case_eq (f2 b); intros;
+  rewrite H0 in H1.
+  case_eq (combineOpt (List.map f2 l) ); intros;
+  rewrite H4 in H1.
+  inversion H1; clear H1; subst.
+  erewrite H; eauto.
+  rewrite H0.
+  erewrite IHls1; eauto.
+  discriminate.
+  discriminate.
+  discriminate.
+  discriminate.
+  
+Qed.
+
+Theorem decrExp_plus : forall x y a b,
+  decrExp a x = Some y -> 
+  decrExp (a + b) x = decrExp b y.
+
+  intros.
+  unfold decrExp in *.
+  destruct x.
+  destruct (le_dec a n ).
+  inversion H; clear H; subst.
+  destruct (le_dec (a + b) n).  
+  destruct (Compare_dec.le_dec b (n - a) ).
+  f_equal.
+  f_equal.
+  lia.
+  lia.
+  destruct (Compare_dec.le_dec b (n - a)).
+  lia.
+  reflexivity.
+  discriminate.
+  inversion H; clear H; subst.
+  reflexivity.
+
+Qed.
+
+Theorem decrExpLs_plus : forall x y a b,
+  decrExpLs a x = Some y -> 
+  decrExpLs (a + b) x = decrExpLs b y.
+
+  induction x; intros; simpl in *.
+  inversion H; clear H; subst.
+  reflexivity.
+
+  optSomeInv.
+  simpl in *.
+  erewrite IHx; eauto.
+  erewrite decrExp_plus.
+  reflexivity.
+  eauto.
+Qed.
+
+Theorem decrExpsLs_app : forall d ls1 ls2 x,
+  decrExpsLs d (ls1 ++ ls2) = Some x ->
+  exists x1 x2 x3,
+    decrExpsLs d ls1 = Some x1 /\
+    decrExpsLs d ls2 = Some x2 /\
+    combineOpt (List.map (decrExpLs ((List.length ls1) * d)) x2) = Some x3 /\
+    x = x1 ++ x3.
+
+  induction ls1; intros; simpl in *.
+  econstructor.
+  econstructor.
+  econstructor.
+  intuition idtac.
+  eauto.
+  erewrite (List.map_ext _ (fun x => Some x)).
+  eapply combineOpt_id.
+  eapply decrExpLs_0.
+
+  case_eq (decrExpsLs d (ls1 ++ ls2)); intros;
+  rewrite H0 in H.
+  case_eq (combineOpt (List.map (decrExpLs d) l) ); intros;
+  rewrite H1 in H.
+  inversion H; clear H; subst.
+  edestruct IHls1; eauto.
+  destruct H.
+  destruct H.
+  intuition idtac; subst.
+  rewrite H2.
+  rewrite map_app in *.
+  rewrite combineOpt_app in *.
+  case_eq (combineOpt (List.map (decrExpLs d) x) ); intros;
+  rewrite H4 in H1.
+  case_eq (combineOpt (List.map (decrExpLs d) x1)); intros;
+  rewrite H5 in H1.
+  inversion H1; clear H1; subst.
+  econstructor.
+  econstructor.
+  econstructor.
+  intuition idtac.
+  eauto.
+
+  erewrite combineOpt_map_map; [
+  reflexivity | idtac | eauto | eauto].
+  intros.
+  rewrite Coq.Arith.Plus.plus_comm.
+  eapply decrExpLs_plus.
+  eauto.
+
+  discriminate.
+  discriminate.
+  discriminate.
+  discriminate.
+
+Qed.
+
+
+Theorem signedWindowsToProg_length : forall ws n,
+  length (signedWindowsToProg ws n) = length ws.
+
+  induction ws; intros; simpl in *. 
+  reflexivity.
+  f_equal.
+  eauto.
+
+Qed.
+
+Theorem signedWindowsToProg_AddProg : forall ws n,
+  AddProg (signedWindowsToProg ws n).
+
+  induction ws; intros; unfold AddProg in *; simpl in *.
+  econstructor.
+  econstructor.
+  trivial.
+  eapply IHws.
+
+Qed.
+
+Theorem decrExpLs_app : forall ls1 ls2 d ls1' ls2',
+  decrExpLs d ls1 = Some ls1' ->
+  decrExpLs d ls2 = Some ls2' ->
+  decrExpLs d (ls1 ++ ls2) = Some (ls1' ++ ls2').
+
+  induction ls1; intros; simpl in *.
+  inversion H; clear H; subst.
+  simpl in *.
+  trivial.
+  case_eq (decrExpLs d ls1); intros.
+  rewrite H1 in H.
+  case_eq (decrExp d a); intros.
+  rewrite H2 in H.
+  inversion H; clear H; subst.
+  erewrite IHls1.
+  reflexivity.
+  trivial.
+  trivial.
+  rewrite H2 in H.
+  discriminate.
+  rewrite H1 in H.
+  destruct (decrExp d a).
+  discriminate.
+  discriminate.
+
+Qed.
+
+Theorem combineOpt_map : forall (A B : Type)(f : A -> B) x y,
+  combineOpt x = Some y ->
+  combineOpt (map (fun z => match z with | Some a => Some (f a) | None => None end) x) = Some (map f y).
+
+  induction x; intros; simpl in *.
+  inversion H; clear H; subst.
+  reflexivity.
+
+  destruct a; simpl in *.
+  case_eq (combineOpt x); intros.
+  rewrite H0 in H.
+  inversion H; clear H; subst.
+  erewrite IHx; eauto.
+  reflexivity.
+  rewrite H0 in H.
+  discriminate.
+  discriminate.
+
+Qed.
+
+Theorem combineOpt_In_not_None : forall (A : Type)(ls : list (option A)) a y,
+  combineOpt ls = Some y ->
+  In a ls ->
+  a <> None.
+
+  induction ls; intros; simpl in *.
+  intuition idtac.
+  destruct a.
+  intuition idtac.
+  subst.
+  discriminate.
+  subst.
+  case_eq (combineOpt ls); intros.
+  rewrite H0 in H.
+  inversion H; clear H; subst.
+  eapply IHls.
+  eauto.
+  eauto.
+  trivial.
+  rewrite H0 in H.
+  discriminate.
+  discriminate.
+
+Qed.
+
+Theorem permuteAndDouble_grouped_cons : forall a perm ws d ls,
+  permuteAndDouble_grouped ws d (a :: perm) = Some ls ->
+  exists ls1 a1 ls2 , permuteAndDouble_grouped ws d perm = Some ls1 /\
+  multiSelect (signedWindowsToProg ws 0) a = Some a1 /\
+  combineOpt (map (decrExpLs d) ls1) = Some ls2 /\
+  ls = (a1 ++ (wm_Double d):: nil)  :: ls2.
+  
+  intros.
+  unfold permuteAndDouble_grouped in *.
+  simpl in *.
+  case_eq (multiSelect (signedWindowsToProg ws 0) a ); intros.
+  rewrite H0 in H.
+  case_eq (combineOpt (map (multiSelect (signedWindowsToProg ws 0)) perm)); intros.
+  rewrite H1 in H.
+  simpl in *.
+  case_eq (decrExpsLs d l0); intros.
+  rewrite H2 in H.
+  
+  case_eq (combineOpt (map (decrExpLs d) l1)); intros.
+  rewrite H3 in H.
+  inversion H; clear H; subst.
+  exists (map
+ (fun x : list WindowedMultOp => x ++ wm_Double d :: nil)
+ l1) .
+  exists l.
+  exists (map
+    (fun x : list WindowedMultOp =>
+     x ++ wm_Double d:: nil) l2).
+  intuition idtac.
+  rewrite <- (combineOpt_map (fun x : list WindowedMultOp => x ++ wm_Double d :: nil) (map (decrExpLs d) l1)); trivial.
+  f_equal.
+  repeat rewrite map_map.
+  eapply map_ext_in_iff.
+  intros.
+  case_eq (decrExpLs d a0); intros. 
+  erewrite decrExpLs_app; simpl; eauto.
+  exfalso.
+  eapply combineOpt_In_not_None;[eapply H3 | idtac | eapply H4].
+  eapply in_map_iff.
+  econstructor.
+  intuition idtac.
+
+  rewrite H3 in H.
+  discriminate.
+  rewrite H2 in H.
+  discriminate.
+  rewrite H1 in H.
+  discriminate.
+  rewrite H0 in H.
+  discriminate.
+Qed.
+
+Theorem combineOpt_map_comm : forall (A : Type)(g : A -> A)(f : A -> option A) x y,
+  (forall a b, f (g a) = Some b -> exists c, (f a) = Some c /\ (g c) = b) -> 
+  combineOpt (map f (map g x)) = Some y ->
+  exists z, combineOpt (map f x) = Some z /\ y = map g z.
+
+  induction x; intros; simpl in *.
+  inversion H0; clear H0; subst.
+  exists nil. intuition idtac.
+  case_eq (f (g a)); intros.
+  rewrite H1 in H0.
+  case_eq (combineOpt (map f (map g x))); intros.
+  rewrite H2 in H0.
+  inversion H0; clear H0; subst.
+  edestruct IHx; eauto.
+  intuition idtac.
+  subst.
+  edestruct H; eauto.
+  intuition idtac; subst.
+  rewrite H4.
+  rewrite H3.
+  econstructor.
+  intuition idtac.
+  rewrite H2 in H0.
+  discriminate.
+  rewrite H1 in H0.
+  discriminate.
+Qed.
+
+Theorem decrExpLs_app_if : forall d x y z,
+  decrExpLs d (x ++ y) = Some z ->
+  exists a b, decrExpLs d x = Some a /\ decrExpLs d y = Some b /\ z = a ++ b.
+
+  induction x; intros; simpl in *.
+  exists nil, z.
+  intuition idtac.
+  case_eq (decrExp d a); intros;
+  rewrite H0 in H.
+  case_eq (decrExpLs d (x++y)); intros;
+  rewrite H1 in H.
+  inversion H; clear H; subst.
+  edestruct IHx; eauto.
+  destruct H.
+  intuition idtac; subst.
+  rewrite H2.
+  econstructor; econstructor; intuition eauto.
+  discriminate.
+  discriminate.
+
+Qed.
+
+Theorem permuteAndDouble_grouped_cons_if : forall a perm ws d ls1 a1 ls2,
+  permuteAndDouble_grouped ws d perm = Some ls1 ->
+  multiSelect (signedWindowsToProg ws 0) a = Some a1 ->
+  combineOpt (map (decrExpLs d) ls1) = Some ls2 ->
+  permuteAndDouble_grouped ws d (a :: perm) = Some ((a1 ++ (wm_Double d):: nil)  :: ls2).
+
+  intros.
+  unfold permuteAndDouble_grouped in *.
+  simpl.
+  rewrite H0.
+  case_eq (combineOpt (map (multiSelect (signedWindowsToProg ws 0)) perm)); intros;
+  rewrite H2 in H.
+  simpl.
+  case_eq (decrExpsLs d l); intros;
+  rewrite H3 in H.
+  inversion H; clear H; subst.
+  apply combineOpt_map_comm in H1.
+  destruct H1.
+  intuition idtac.
+  subst.
+  rewrite H1.
+  simpl.
+  reflexivity.
+
+  intros.
+  edestruct decrExpLs_app_if; eauto.
+  destruct H4.
+  intuition idtac; subst.
+  inversion H4; clear H4; subst.
+  econstructor.
+  intuition idtac; eauto.
+  discriminate.
+  discriminate.
+Qed.
+
+Theorem multiSelect_cons : forall (A : Type)(x : list A) y1 y2,
+  multiSelect x (y1 :: y2) = 
+  match (nth_error x y1) with
+  | Some y1' =>
+    match (multiSelect x y2) with
+    | Some y2' => Some (y1' :: y2')
+    | None => None
+    end
+  | None => None
+  end. 
+  
+  intros.
+  reflexivity.
+
+Qed.
+
+Theorem multiSelect_app : forall (A : Type)(x : list A) y1 y2,
+  multiSelect x (y1 ++ y2) = 
+  match (multiSelect x y1) with
+  | Some y1' => 
+    match (multiSelect x y2) with 
+    | Some y2' =>  Some (y1' ++ y2')
+    | None => None
+    end
+  | None => None
+   end.
+
+  induction y1; intros; simpl in *.
+  destruct (multiSelect x y2); trivial.
+  repeat rewrite multiSelect_cons.
+  rewrite IHy1.
+  case_eq (nth_error x a); intros.
+  case_eq (multiSelect x y1); intros.
+  case_eq (multiSelect x y2); intros.
+  simpl.
+  reflexivity.
+  reflexivity.
+  reflexivity.
+  reflexivity.
+
+Qed.
+
+Theorem insertDoubleAt_0 : forall d l1,
+  insertDoubleAt d l1 0 = insertDouble d l1.
+
+  induction l1; intros; simpl in *;
+  reflexivity.
+
+Qed.
+
+Theorem insertDoubleAt_app : forall l0 l1 d x,
+  insertDoubleAt d (l0 ++ l1) (length l0)  = Some x ->
+  exists y, decrExpLs d l1 = Some y /\
+  x = (l0 ++ (wm_Double d):: y).
+
+  induction l0; intros; simpl in *.
+  rewrite insertDoubleAt_0 in H.
+  unfold insertDouble in *.
+  case_eq (decrExpLs d l1); intros.
+  rewrite H0 in H.
+  inversion H; clear H; subst.
+  econstructor; eauto.
+  rewrite H0 in H.
+  discriminate.
+  case_eq (insertDoubleAt d (l0 ++ l1) (length l0) ); intros;
+  rewrite H0 in H.
+  inversion H; clear H; subst.
+  edestruct IHl0; eauto.
+  intuition idtac.
+  subst.
+  exists x.
+  intuition idtac.
+  discriminate.
+
+Qed.
+
+Theorem insertDoubleAt_ge : forall a l0 l1 d l,
+  (a >= length l0)%nat ->
+  insertDoubleAt d (l0 ++ l1) a = Some l ->
+  exists b l2, insertDoubleAt d l1 b = Some l2 /\
+  l = l0 ++ l2 /\ (a = (length l0) + b)%nat.
+
+  induction a; intros; simpl in *.
+  rewrite insertDoubleAt_0 in *.
+  replace l0 with (@nil WindowedMultOp) in *.
+  simpl in *.
+  exists 0%nat.
+  exists l.
+  rewrite insertDoubleAt_0 in *.
+  intuition idtac.
+  destruct l0; simpl in *; trivial.
+  lia.
+
+  destruct l0; simpl in *.
+  exists (S a).
+  exists l.
+  intuition idtac.
+  case_eq (insertDoubleAt d (l0 ++ l1) a); intros;
+  rewrite H1 in H0.
+  inversion H0; clear H0; subst.
+  edestruct (IHa l0).
+  lia.
+  eauto.
+  destruct H0.
+  intuition idtac; subst.
+  exists x.
+  exists x0.
+  intuition idtac.
+  discriminate.
+
+Qed.
+
+
+Theorem insertDoubleAt_app_if : forall l0 l1 d x0 x,
+  insertDoubleAt d l1 x0 = Some x -> 
+  insertDoubleAt d (l0 ++ l1) (length l0 + x0) = Some (l0 ++ x).
+
+  induction l0; intros; simpl in *.
+  trivial.
+  erewrite IHl0.
+  reflexivity.
+  trivial.
+
+Qed.
+
+
+Theorem insertDoublesAt_app : forall lsn d l0 l1 x,
+  (forall n, In n lsn -> n >= length l0)%nat ->
+  insertDoublesAt d (l0 ++ l1) (lsn ++ length l0 :: nil)  = Some x -> 
+  exists y z, 
+  (insertDoublesAt d l1 (map (fun x => minus x (length l0)) lsn)) = Some y /\
+  decrExpLs d y = Some z /\
+  x = l0 ++ (wm_Double d)::z.
+
+  induction lsn; intros; simpl in *.
+  case_eq (insertDoubleAt d (l0 ++ l1) (length l0)); intros.
+  rewrite H1 in H0.
+  inversion H0; clear H0; subst.
+  edestruct insertDoubleAt_app; eauto.
+  rewrite H1 in H0.
+  discriminate.
+
+  case_eq (insertDoubleAt d (l0 ++ l1) a); intros.
+  rewrite H1 in H0.
+  apply insertDoubleAt_ge in H1.
+  destruct H1.
+  destruct H1.
+  intuition idtac; subst.
+  edestruct (IHlsn d l0).
+  intuition idtac.
+  eapply H.
+  intuition idtac.
+  eauto.
+  destruct H1.
+  intuition idtac; subst.
+  rewrite minus_plus.
+  rewrite H2.
+ 
+  exists x2.
+  exists x3.
+  intuition idtac.
+  eapply H.
+  intuition idtac.
+  
+  rewrite H1 in H0.
+  discriminate.
+
+Qed.
+
+Theorem insertDoublesAt_app_if : forall lsn d l0 l1 y z,
+  (forall n, In n lsn -> n >= length l0)%nat ->
+  (insertDoublesAt d l1 (map (fun x => minus x (length l0)) lsn)) = Some y ->
+  decrExpLs d y = Some z ->
+   insertDoublesAt d (l0 ++ l1) (lsn ++ length l0 :: nil)  = Some (l0 ++ (wm_Double d)::z).
+
+  induction lsn; intros; simpl in *.
+  inversion H0; clear H0; subst.
+  replace (length l0) with (length l0 + 0)%nat.
+  erewrite insertDoubleAt_app_if.
+  reflexivity.
+  rewrite insertDoubleAt_0.
+  unfold insertDouble.
+  rewrite H1.
+  reflexivity.
+  lia.
+  
+  case_eq (insertDoubleAt d l1 (a - length l0) ); intros;
+  rewrite H2 in H0.
+  replace a with (length l0 + (a - length l0))%nat.
+  erewrite insertDoubleAt_app_if.
+  eapply IHlsn.
+  intros.
+  eapply H.
+  intuition idtac.
+  eauto.
+  trivial.
+  trivial.
+  specialize (H a).
+  intuition idtac.
+  lia.
+  discriminate.
+
+Qed.
+
+Theorem endIndices_h_map_sub : forall (A : Type)(ls : list (list A)) x y,
+  (y <= x)%nat ->
+  map (fun n => minus n y) (endIndices_h ls x) = endIndices_h ls (minus x y).
+
+  induction ls; intros; simpl in *.
+  reflexivity.
+  f_equal.
+  lia.
+  rewrite IHls.
+  f_equal.
+  lia.
+  lia.
+
+Qed.
+
+Theorem In_endIndices_h_ge : forall (A : Type)(ls : list (list A)) n m,
+  In n (endIndices_h ls m) ->
+  (n >= m)%nat.
+
+  induction ls; intros; simpl in *.
+  intuition idtac.
+  intuition idtac; subst.
+  lia.
+  eapply le_trans; [idtac |
+  eapply IHls; eauto].
+  lia.
+
+Qed.
+
+Theorem combineOpt_length : forall (A : Type)(ls : list (option A)) x,
+  combineOpt ls = Some x ->
+  length ls = length x.
+
+  induction ls; intros; simpl in *.
+  inversion H; clear H; subst.
+  trivial.
+  destruct a.
+  case_eq (combineOpt ls); intros;
+  rewrite H0 in H.
+  inversion H; clear H; subst.
+  simpl.
+  f_equal; eauto.
+  discriminate.
+  discriminate.
+
+Qed.
+
+Theorem multiSelect_length : forall (A : Type)(ls : list A) a b,
+  multiSelect ls a = Some b ->
+  length a = length b.
+
+  intros.
+  unfold multiSelect in *.
+  apply combineOpt_length in H.
+  rewrite map_length in H.
+  trivial.
+
+Qed.
+
+Theorem permuteAndDouble_flatten_app_cons : forall  ws d a perm x,
+  permuteAndDouble ws d (a ++ flatten perm) (endIndices (a :: perm))  = Some x ->
+  exists a1 x1 x2, multiSelect (signedWindowsToProg ws 0) a = Some a1 /\
+  permuteAndDouble ws d (flatten perm) (endIndices perm) = Some x1 /\
+  decrExpLs d x1 = Some x2 /\
+  x = a1 ++ (wm_Double d)::x2.
+
+  intros.
+  unfold permuteAndDouble in *.
+  case_eq (multiSelect (signedWindowsToProg ws 0) (a ++ flatten perm)); intros.
+  rewrite H0 in H.
+  rewrite multiSelect_app in *.
+  case_eq (multiSelect (signedWindowsToProg ws 0) a); intros.
+  rewrite H1 in H0.
+  exists l0.
+  case_eq (multiSelect (signedWindowsToProg ws 0) (flatten perm) ); intros.
+  rewrite H2 in H0.
+  inversion H0; clear H0; subst.
+  unfold endIndices in *.
+  simpl in *.
+  rewrite plus_0_r in *.
+  replace (length a) with (length l0) in H.
+  apply insertDoublesAt_app in H.
+  destruct H.
+  destruct H.
+  intuition idtac. subst.
+  rewrite map_rev in *.
+  rewrite endIndices_h_map_sub in *.
+  rewrite minus_diag in *.
+  exists x0.
+  exists x1.
+  intuition idtac.
+  lia.
+
+  intros.
+  apply in_rev in H0.
+  eapply In_endIndices_h_ge; eauto.
+  symmetry.
+  eapply multiSelect_length; eauto.
+  rewrite H2 in H0.
+  discriminate.
+  rewrite H1 in H0.
+  discriminate.
+  rewrite H0 in H.
+  discriminate.
+
+Qed.
+
+Theorem permuteAndDouble_flatten_app_cons_if : forall  ws d a perm a1 x1 x2,
+  multiSelect (signedWindowsToProg ws 0) a = Some a1 ->
+  permuteAndDouble ws d (flatten perm) (endIndices perm) = Some x1 -> 
+  decrExpLs d x1 = Some x2 -> 
+  permuteAndDouble ws d (a ++ flatten perm) (endIndices (a :: perm))  = Some (a1 ++ (wm_Double d)::x2).
+
+  intros.
+  unfold permuteAndDouble in *.
+  case_eq (multiSelect (signedWindowsToProg ws 0) (flatten perm) ); intros.
+  rewrite H2 in H0.
+  rewrite multiSelect_app.
+  rewrite H2.
+  rewrite H.
+  unfold endIndices. simpl.
+  rewrite plus_0_r.
+  replace (length a) with (length a1).
+  erewrite insertDoublesAt_app_if.
+  reflexivity.
+  intros.
+  eapply In_endIndices_h_ge.
+  eapply in_rev.
+  eauto.
+  rewrite map_rev.
+  erewrite endIndices_h_map_sub.
+  rewrite minus_diag.
+  eapply H0.
+  lia.
+  trivial.
+  symmetry.
+  eapply multiSelect_length.
+  eauto.
+  rewrite H2 in H0.
+  discriminate.
+  
+Qed.
+
+Theorem combineOpt_map_flatten : 
+  forall (A B : Type)(f : list A -> option (list B)) x x1,
+  combineOpt (map f x) = Some x1 ->
+  f nil = Some nil ->
+  (forall a b y z, f a = Some y -> f b = Some z -> f (a ++ b) = Some (y ++ z)) -> 
+  f (flatten x) = Some (flatten x1).
+
+  induction x; intros; simpl in *.
+  inversion H; clear H; subst.
+  simpl.  
+  trivial.
+
+  case_eq (f a); intros;
+  rewrite H2 in H.
+  case_eq (combineOpt (map f x)); intros;
+  rewrite H3 in H.
+  inversion H; clear H; subst.
+  simpl.
+  erewrite H1.
+  eauto.
+  trivial.
+  eapply IHx;
+  eauto.
+  
+  discriminate.
+  discriminate.
+
+Qed.
+
+    
+Theorem permuteAndDouble_grouped_equiv : forall perm ws d ls,
+  permuteAndDouble_grouped ws d perm = Some ls ->
+  permuteAndDouble ws d (flatten perm) (endIndices perm) = Some (flatten ls).
+
+  induction perm; intros; simpl in *.
+  inversion H; clear H; subst.
+  reflexivity.
+  apply permuteAndDouble_grouped_cons in H.
+  destruct H.
+  destruct H.
+  destruct H.
+  intuition idtac; subst.
+  apply IHperm in H0.
+  simpl.
+  erewrite permuteAndDouble_flatten_app_cons_if.
+  replace ((x0 ++ wm_Double d :: nil) ++ flatten x1) with (x0 ++ wm_Double d :: (flatten x1)).
+  reflexivity.
+  rewrite <- app_assoc.
+  simpl.
+  reflexivity.
+  trivial.
+  eauto.
+  eapply combineOpt_map_flatten in H1.
+  trivial.
+  reflexivity.
+  intros.
+  eapply decrExpLs_app; eauto.
+
+Qed.
+
+
+Definition stripOptLs(A : Type)(x: option (list A)) :=
+  match x with
+  | Some y => y
+  | None => nil
+  end. 
+
+
+Theorem decrExpLs_flatten : forall d x2 x1,
+  decrExpLs d (flatten x2) = Some x1 ->
+  flatten (map (fun x => stripOptLs (decrExpLs d x)) x2) = x1.
+
+  induction x2; intros; simpl in *.
+  inversion H; clear H; subst.
+  reflexivity.
+  apply decrExpLs_app_if in H.
+  destruct H.
+  destruct H.
+  intuition idtac; subst.
+  apply IHx2 in H.
+  subst.
+  f_equal.
+  rewrite H0.
+  reflexivity.
+
+Qed.
+
+Theorem decrExpLs_combineOpt : forall d x2 x1,
+  decrExpLs d (flatten x2) = Some x1 ->
+  combineOpt (map (decrExpLs d) x2) =
+  Some (map (fun x0 : list WindowedMultOp => stripOptLs (decrExpLs d x0)) x2).
+
+  induction x2; intros; simpl in *.
+  reflexivity.
+  apply decrExpLs_app_if in H.
+  destruct H.
+  destruct H.
+  intuition idtac; subst.
+  rewrite H0.
+  erewrite IHx2; eauto.
+  
+Qed.
+
+Theorem permuteAndDouble_grouped_equiv_if : forall perm ws d ls,
+  permuteAndDouble ws d (flatten perm) (endIndices perm) = Some ls -> 
+  exists ls', permuteAndDouble_grouped ws d perm = Some ls' /\ flatten ls' = ls.
+
+  induction perm; intros; simpl in *.
+  unfold permuteAndDouble in *.
+  simpl in *.
+  inversion H; clear H; subst.
+  exists nil.
+  intuition idtac.
+  apply permuteAndDouble_flatten_app_cons in H.
+  destruct H.
+  destruct H.
+  destruct H.
+  intuition idtac.
+  subst.
+  apply IHperm in H.
+  destruct H.
+  intuition idtac; subst.
+  erewrite (@permuteAndDouble_grouped_cons_if _ _ _ _ _ x (map (fun x => stripOptLs (decrExpLs d x)) x2)); eauto.
+  econstructor.
+  intuition idtac; eauto.
+  simpl.
+  rewrite <- app_assoc.
+  f_equal.
+  simpl.
+  f_equal.
+  eapply decrExpLs_flatten; eauto.
+  eapply decrExpLs_combineOpt; eauto.
+  
+Qed.
+
+
+Section MachineEval.
+
+  Variable GroupElem : Type.
+  
+  Context `{GroupElem_eq : Setoid GroupElem}.
+
+  Variable groupAdd : GroupElem -> GroupElem -> GroupElem.
+  Hypothesis groupAdd_proper : Proper (equiv ==> equiv ==> equiv) groupAdd.
+
+  Hypothesis groupAdd_assoc : forall a b c,
+    groupAdd (groupAdd a b) c == groupAdd a (groupAdd b c).
+  Hypothesis groupAdd_comm : forall a b,
+    groupAdd a b == groupAdd b a.
+
+  Variable idElem : GroupElem.
+  Hypothesis groupAdd_id : forall x, groupAdd idElem x == x.
+
+  Variable groupDouble : GroupElem -> GroupElem.
+  Hypothesis groupDouble_proper : Proper (equiv ==> equiv) groupDouble.
+  Hypothesis groupDouble_correct : forall x,
+    groupDouble x == groupAdd x x.
+
+  Variable groupInverse : GroupElem -> GroupElem.
+  Hypothesis groupInverse_proper : Proper (equiv ==> equiv) groupInverse.
+  Hypothesis groupInverse_id : groupInverse idElem == idElem.
+  Hypothesis groupInverse_correct : forall e, groupAdd e (groupInverse e) == idElem.
+  Hypothesis groupInverse_add_distr : forall e1 e2, groupInverse (groupAdd e1 e2) == groupAdd (groupInverse e1) (groupInverse e2).
+  Hypothesis groupInverse_involutive : forall e, groupInverse (groupInverse e) == e.
+
+  Variable p : GroupElem.
+  Variable RegularWindow : SignedWindow -> Prop.
+
+  Variable wsize : nat.
+  Hypothesis wsize_nz : wsize <> 0%nat.
+
+  Definition groupMul_doubleAdd_signed := groupMul_doubleAdd_signed groupAdd idElem groupDouble groupInverse.
+
+  Variable bMultiple : SignedWindow -> GroupElem.
+  Hypothesis bMultiple_correct : forall w, 
+    RegularWindow w ->
+    bMultiple w == groupMul_doubleAdd_signed w p.
+
+  Definition groupMul_signedWindows := groupMul_signedWindows groupAdd idElem groupDouble wsize bMultiple.
+  Definition groupMul_signedWindows_exp := groupMul_signedWindows_exp groupAdd idElem groupDouble groupInverse wsize p.
+  Definition groupDouble_n := groupDouble_n groupDouble.
+
+  Definition evalWindowMult (m : WindowedMultOp)(e : GroupElem) :=
+    match m with
+    | wm_Add n w => (groupAdd (groupMul_doubleAdd_signed (zDouble_n (n * wsize) w) p) e)
+    | wm_Double n => (groupDouble_n (n * wsize) e)
+    end.
+
+  Theorem evalWindowMult_compat : forall m e1 e2,
+    e1 == e2 ->
+    evalWindowMult m e1 == evalWindowMult m e2.
+
+    intros.
+    unfold evalWindowMult.
+    destruct m.
+    apply groupAdd_proper.
+    reflexivity.
+    trivial.
+    apply groupDouble_n_equiv_compat;
+    trivial.
+
+  Qed.
+
+  Fixpoint groupMul_signedWindows_prog (ws : list WindowedMultOp) : GroupElem :=
+    match ws with
+    | nil => idElem
+    | w :: ws' => evalWindowMult w (groupMul_signedWindows_prog ws')
+    end.
+
+  Theorem groupMul_signedWindows_prog_equiv : forall ws n,
+    groupMul_signedWindows_prog (signedWindowsToProg ws n) == groupMul_signedWindows_exp ws n.
+
+    induction ws; intros; simpl in *.
+    reflexivity.
+    rewrite IHws.
+    reflexivity.
+
+  Qed.
+
+  Theorem evalWindowMult_double_equiv : forall n a w e,
+    (decrExp n a) = Some w ->
+    evalWindowMult a (groupDouble_n (n * wsize) e) == groupDouble_n (n * wsize) (evalWindowMult w e).
+
+    intros.
+    unfold decrExp, evalWindowMult in *.
+    destruct a.
+    destruct (le_dec n n0).
+    inversion H; clear H; subst.
+    unfold groupMul_doubleAdd_signed.
+    rewrite zDouble_n_mul; eauto.
+    assert (exists m, n + m = n0)%nat.
+    exists (n0 - n)%nat.
+    lia.
+    destruct H. subst.
+    rewrite Nat.mul_add_distr_r.
+    rewrite groupDouble_n_add.
+    rewrite groupAdd_groupDouble_n_distr; eauto.
+    apply groupDouble_n_equiv_compat; eauto.
+    apply groupAdd_proper.
+    rewrite zDouble_n_mul; eauto.
+    replace (n + x - n)%nat with x.
+    reflexivity.
+    lia.
+    reflexivity.
+    discriminate.
+
+    inversion H; clear H; subst.  
+    unfold groupDouble_n.
+    rewrite <- groupDouble_n_add.
+    rewrite plus_comm.
+    rewrite groupDouble_n_add.
+    reflexivity.
+
+  Qed.
+
+  Theorem insertDouble_equiv_h : forall n ps ps',
+    Some ps' = decrExpLs n ps ->
+    groupMul_signedWindows_prog ps == groupDouble_n (n * wsize) (groupMul_signedWindows_prog ps').
+
+    induction ps; intros; simpl in *.
+    inversion H; clear H; subst.
+    simpl.
+    unfold groupDouble_n.
+    rewrite groupDouble_n_id; eauto.
+    reflexivity.
+    remember (decrExp n a) as z1. destruct z1.
+    remember (decrExpLs n ps) as z2. destruct z2.
+    inversion H; clear H; subst.
+    simpl.
+    transitivity (evalWindowMult a (groupDouble_n (n * wsize) (groupMul_signedWindows_prog l))).
+    eapply evalWindowMult_compat; eauto.
+    eapply evalWindowMult_double_equiv.
+    symmetry.
+    trivial.
+    discriminate.
+    discriminate.
+  Qed.
+
+  Theorem insertDouble_equiv : forall n ps ps',
+    (insertDouble n ps) = Some ps' -> 
+    groupMul_signedWindows_prog ps == groupMul_signedWindows_prog ps'.
+
+    intros.
+    unfold insertDouble in *.
+    remember (decrExpLs n ps) as z.
+    destruct z.
+    inversion H; clear H; subst.
+    simpl.
+    eapply insertDouble_equiv_h; eauto.
+    discriminate.
+  Qed.
+
+  Theorem swapFront_equiv_h : forall w w0 w1 w2 ps,
+    Some (w1, w2) = swapPair w w0 ->
+    groupMul_signedWindows_prog (w :: w0 :: ps) == groupMul_signedWindows_prog (w1 :: w2 :: ps).
+
+    intros.
+    simpl.
+    unfold swapPair in *.
+    destruct w.
+    destruct w0.
+    inversion H; clear H; subst.  
+    unfold evalWindowMult. 
+    repeat rewrite <- groupAdd_assoc.
+    apply groupAdd_proper.
+    apply groupAdd_comm.
+    reflexivity.
+
+    destruct (le_dec n0 n).
+    inversion H; clear H; subst.
+    assert (exists n1, n1 + n0 = n)%nat.
+    exists (n - n0)%nat.
+    lia.
+    destruct H.
+    subst.
+    replace (x + n0 - n0)%nat with x.
+    unfold evalWindowMult.
+    unfold groupMul_doubleAdd_signed.
+    rewrite zDouble_n_mul; eauto.
+    rewrite Nat.mul_add_distr_r.
+    rewrite plus_comm.
+    rewrite groupDouble_n_add.
+    rewrite groupAdd_groupDouble_n_distr; eauto.
+    apply groupDouble_n_equiv_compat; eauto.
+    apply groupAdd_proper.
+    rewrite zDouble_n_mul; eauto.
+    reflexivity.
+    reflexivity.
+    lia.
+    discriminate.
+
+    destruct w0.
+    inversion H; clear H; subst.
+    unfold evalWindowMult.
+    symmetry.
+    unfold groupMul_doubleAdd_signed.
+    rewrite zDouble_n_mul; eauto.
+    rewrite Nat.mul_add_distr_r.
+    rewrite groupDouble_n_add.
+    rewrite groupAdd_groupDouble_n_distr; eauto.
+    apply groupDouble_n_equiv_compat; eauto.
+    apply groupAdd_proper.
+    rewrite zDouble_n_mul; eauto.
+    reflexivity.
+    reflexivity.
+
+    inversion H; clear H; subst.
+    unfold evalWindowMult.
+    unfold groupDouble_n.
+    rewrite <- groupDouble_n_add; eauto.
+    rewrite plus_comm.
+    rewrite groupDouble_n_add.
+    reflexivity.
+
+  Qed.
+
+  Theorem swapFront_equiv : forall ps ps',
+    (swapFront ps) = Some ps' -> 
+    groupMul_signedWindows_prog ps == groupMul_signedWindows_prog ps'.
+
+    intros.
+    unfold swapFront in *.
+    destruct ps.
+    discriminate.
+    destruct ps.
+    discriminate.
+    remember (swapPair w w0) as z.
+    destruct z.
+    destruct p0.
+    inversion H; clear H; subst.
+    simpl.
+    apply swapFront_equiv_h.
+    trivial.
+    discriminate.
+
+  Qed.
+
+  Theorem addProgPermEq : forall (ps1 ps2 : list WindowedMultOp),
+    Permutation ps1 ps2 ->
+    AddProg ps1 ->
+    groupMul_signedWindows_prog ps1 == groupMul_signedWindows_prog ps2.
+
+    induction 1; intros; simpl in *.
+    reflexivity.
+
+    apply evalWindowMult_compat.
+    eapply IHPermutation.
+    inversion H0; eauto.
+    inversion H; clear H; subst.
+    inversion H3; clear H3; subst.
+    
+    unfold evalWindowMult.
+    destruct y.
+    destruct x.
+    repeat rewrite <- groupAdd_assoc.
+    apply groupAdd_proper.
+    rewrite groupAdd_comm.
+    reflexivity.
+    reflexivity.
+    intuition idtac.
+    intuition idtac.
+
+    rewrite IHPermutation1.
+    apply IHPermutation2.
+    eauto.
+    eapply Permutation_Forall.
+    eauto.
+    eauto.
+    eauto.
+
+  Qed.
+
+  Theorem insertDoubleAt_equiv : forall n d ls ls',
+    insertDoubleAt d ls n = Some ls' ->
+    groupMul_signedWindows_prog ls == groupMul_signedWindows_prog ls'.
+
+    induction n; intros; simpl in *.
+    replace (insertDoubleAt d ls 0) with (insertDouble d ls) in H.
+    eapply insertDouble_equiv.
+    eauto.
+    destruct ls; simpl in *.
+    reflexivity.
+    reflexivity.
+    
+    destruct ls; simpl in *.
+    discriminate.
+    case_eq (insertDoubleAt d ls n); intros;
+    rewrite H0 in H.
+    inversion H; clear H; subst.
+    simpl.
+    apply evalWindowMult_compat.
+    eapply IHn.
+    eauto.
+    discriminate.
+
+  Qed.
+
+  Theorem insertDoublesAt_equiv : forall lsn d ls ls',
+    insertDoublesAt d ls lsn = Some ls' ->
+    groupMul_signedWindows_prog ls == groupMul_signedWindows_prog ls'.
+
+    induction lsn; intros; simpl in *.
+    inversion H; clear H; subst.
+    reflexivity.
+    
+    case_eq (insertDoubleAt d ls a); intros;
+    rewrite H0 in H.
+    transitivity (groupMul_signedWindows_prog l).
+    eapply insertDoubleAt_equiv; eauto.
+    eauto.
+    discriminate.
+  Qed.
+
+  Theorem permuteAndDouble_equiv : forall ws d perm doubles ps,
+    Forall RegularWindow ws -> 
+    Permutation perm (seq 0 (length ws)) ->
+    permuteAndDouble ws d perm doubles = Some ps -> 
+    groupMul_signedWindows_prog ps == groupMul_signedWindows ws.
+
+    intros.
+    unfold permuteAndDouble in *.
+    case_eq (multiSelect (signedWindowsToProg ws 0) perm); intros;
+    rewrite H2 in H1.
+    transitivity (groupMul_signedWindows_prog l).
+    symmetry.
+    eapply insertDoublesAt_equiv; eauto.
+    transitivity (groupMul_signedWindows_prog (signedWindowsToProg ws 0) ).
+    symmetry.
+    apply addProgPermEq.
+    eapply multiSelect_perm; [idtac | eauto].
+    rewrite signedWindowsToProg_length.
+    trivial.
+    apply signedWindowsToProg_AddProg.
+    rewrite groupMul_signedWindows_prog_equiv.
+    unfold groupMul_signedWindows_exp.
+    rewrite <- groupMul_signedWindows_exp_equiv; eauto.
+    rewrite Nat.mul_0_r.
+    simpl.
+    reflexivity.
+    trivial.
+    
+    discriminate.
+
+  Qed.
+
+End MachineEval.
